Cleaning up the Haskell interface

opentheory/haskell/parser.ml
@@ -4,167 +4,201 @@
 (* ========================================================================= *)
 
 (* ------------------------------------------------------------------------- *)
-(* Defining Haskell parsers and streams.                                     *)
+(* Definition of Haskell parsers and streams.                                *)
 (* ------------------------------------------------------------------------- *)
 
 logfile "haskell-parser-def";;
 
 (* Streams *)
 
-let is_streamH_def =
-  let def = new_definition
-    `!(s : A stream). is_streamH s <=> T` in
-  REWRITE_RULE [] def;;
-
-let streamH_exists = prove
-  (`?(s : A stream). is_streamH s`,
-   EXISTS_TAC `s : A stream` THEN
-   REWRITE_TAC [is_streamH_def]);;
-
-let (streamH_abs_rep,streamH_rep_abs) =
+let (streamH_lift_drop,streamH_drop_lift) =
+  let exists = prove (`?(s : A stream). T`, REWRITE_TAC []) in
   let tybij =
     new_type_definition
-      "streamH" ("mk_streamH","dest_streamH") streamH_exists in
-  CONJ_PAIR (REWRITE_RULE [is_streamH_def] tybij);;
+      "streamH" ("lift_streamH","drop_streamH") exists in
+  CONJ_PAIR (REWRITE_RULE [] tybij);;
 
-export_thm streamH_abs_rep;;
-export_thm streamH_rep_abs;;
+export_thm streamH_lift_drop;;
+export_thm streamH_drop_lift;;
 
-let streamH_tybij = CONJ streamH_abs_rep streamH_rep_abs;;
+let streamH_tybij = CONJ streamH_lift_drop streamH_drop_lift;;
 
 let ErrorH_def = new_definition
-  `(ErrorH : A streamH) = mk_streamH Error`;;
+  `(ErrorH : A streamH) = lift_streamH Error`;;
 
 export_thm ErrorH_def;;
 
 let EofH_def = new_definition
-  `(EofH : A streamH) = mk_streamH Eof`;;
+  `(EofH : A streamH) = lift_streamH Eof`;;
 
 export_thm EofH_def;;
 
 let StreamH_def = new_definition
-  `!(a : A) s. StreamH a s = mk_streamH (Stream a (dest_streamH s))`;;
+  `!(a : A) s. StreamH a s = lift_streamH (Stream a (drop_streamH s))`;;
 
 export_thm StreamH_def;;
 
 let case_streamH_def = new_definition
   `!(e : B) b f (s : A streamH).
      case_streamH e b f s =
-     case_stream e b (\a t. f a (mk_streamH t)) (dest_streamH s)`;;
+     case_stream e b (\a t. f a (lift_streamH t)) (drop_streamH s)`;;
 
 export_thm case_streamH_def;;
 
 let length_streamH_def = new_definition
-  `!(s : A streamH). length_streamH s = length_stream (dest_streamH s)`;;
+  `!(s : A streamH). length_streamH s = length_stream (drop_streamH s)`;;
 
 export_thm length_streamH_def;;
 
 let stream_to_listH_def = new_definition
-  `!(s : A streamH). stream_to_listH s = stream_to_list (dest_streamH s)`;;
+  `!(s : A streamH). stream_to_listH s = stream_to_list (drop_streamH s)`;;
 
 export_thm stream_to_listH_def;;
 
 let append_streamH_def = new_definition
   `!l (s : A streamH).
-     append_streamH l s = mk_streamH (append_stream l (dest_streamH s))`;;
+     append_streamH l s = lift_streamH (append_stream l (drop_streamH s))`;;
 
 export_thm append_streamH_def;;
 
 let list_to_streamH_def = new_definition
-  `!(l : A list). list_to_streamH l = mk_streamH (list_to_stream l)`;;
+  `!(l : A list). list_to_streamH l = lift_streamH (list_to_stream l)`;;
 
 export_thm list_to_streamH_def;;
 
 (* Parsers *)
 
-let is_parserH_def =
-  let def = new_definition
-    `!(p : (A,B) parser). is_parserH p <=> T` in
-  REWRITE_RULE [] def;;
-
-let parserH_exists = prove
-  (`?(p : (A,B) parser). is_parserH p`,
-   EXISTS_TAC `p : (A,B) parser` THEN
-   REWRITE_TAC [is_parserH_def]);;
-
-let (parserH_abs_rep,parserH_rep_abs) =
+let (parserH_lift_drop,parserH_drop_lift) =
+  let exists = prove (`?(p : (A,B) parser). T`, REWRITE_TAC []) in
   let tybij =
     new_type_definition
-      "parserH" ("mk_parserH","dest_parserH") parserH_exists in
-  CONJ_PAIR (REWRITE_RULE [is_parserH_def] tybij);;
+      "parserH" ("lift_parserH","drop_parserH") exists in
+  CONJ_PAIR (REWRITE_RULE [] tybij);;
 
-export_thm parserH_abs_rep;;
-export_thm parserH_rep_abs;;
+export_thm parserH_lift_drop;;
+export_thm parserH_drop_lift;;
 
-let parserH_tybij = CONJ parserH_abs_rep parserH_rep_abs;;
+let parserH_tybij = CONJ parserH_lift_drop parserH_drop_lift;;
 
-let (mk_parser_resultH_none,mk_parser_resultH_some) =
+let (lift_parser_resultH_none,lift_parser_resultH_some) =
   let def = new_definition
-    `(mk_parser_resultH : (B # A stream) option ->  (B # A streamH) option) =
+    `(lift_parser_resultH : (B # A stream) option ->  (B # A streamH) option) =
        case_option
          NONE
-         (\ (b,s'). SOME (b, mk_streamH s'))` in
+         (\ (b,s'). SOME (b, lift_streamH s'))` in
   let th_none = prove
-    (`mk_parser_resultH (NONE : (B # A stream) option) =
+    (`lift_parser_resultH (NONE : (B # A stream) option) =
       (NONE : (B # A streamH) option)`,
      REWRITE_TAC [def; case_option_def])
   and th_some = prove
     (`!(b : B) (s : A stream).
-         mk_parser_resultH (SOME (b,s)) = SOME (b, mk_streamH s)`,
+         lift_parser_resultH (SOME (b,s)) = SOME (b, lift_streamH s)`,
      REWRITE_TAC [def; case_option_def]) in
   (th_none,th_some);;
 
-export_thm mk_parser_resultH_none;;
-export_thm mk_parser_resultH_some;;
+export_thm lift_parser_resultH_none;;
+export_thm lift_parser_resultH_some;;
 
-let mk_parser_resultH_def =
-    CONJ mk_parser_resultH_none mk_parser_resultH_some;;
+let lift_parser_resultH_def =
+    CONJ lift_parser_resultH_none lift_parser_resultH_some;;
 
-let (dest_parser_resultH_none,dest_parser_resultH_some) =
+let (drop_parser_resultH_none,drop_parser_resultH_some) =
   let def = new_definition
-    `(dest_parser_resultH : (B # A streamH) option ->  (B # A stream) option) =
+    `(drop_parser_resultH : (B # A streamH) option ->  (B # A stream) option) =
        case_option
          NONE
-         (\ (b,s'). SOME (b, dest_streamH s'))` in
+         (\ (b,s'). SOME (b, drop_streamH s'))` in
   let th_none = prove
-    (`dest_parser_resultH (NONE : (B # A streamH) option) =
+    (`drop_parser_resultH (NONE : (B # A streamH) option) =
       (NONE : (B # A stream) option)`,
      REWRITE_TAC [def; case_option_def])
   and th_some = prove
     (`!(b : B) (s : A streamH).
-         dest_parser_resultH (SOME (b,s)) = SOME (b, dest_streamH s)`,
+         drop_parser_resultH (SOME (b,s)) = SOME (b, drop_streamH s)`,
      REWRITE_TAC [def; case_option_def]) in
   (th_none,th_some);;
 
-export_thm dest_parser_resultH_none;;
-export_thm dest_parser_resultH_some;;
+export_thm drop_parser_resultH_none;;
+export_thm drop_parser_resultH_some;;
 
-let dest_parser_resultH_def =
-    CONJ dest_parser_resultH_none dest_parser_resultH_some;;
+let drop_parser_resultH_def =
+    CONJ drop_parser_resultH_none drop_parser_resultH_some;;
 
-let mk_parseH_def = new_definition
+let lift_parser_functionH_def = new_definition
   `!(p : A -> A stream -> (B # A stream) option).
-     mk_parseH p a s = mk_parser_resultH (p a (dest_streamH s))`;;
+     lift_parser_functionH p =
+     \a s. lift_parser_resultH (p a (drop_streamH s))`;;
 
-export_thm mk_parseH_def;;
+export_thm lift_parser_functionH_def;;
 
-let dest_parseH_def = new_definition
+let drop_parser_functionH_def = new_definition
   `!(p : A -> A streamH -> (B # A streamH) option).
-     dest_parseH p a s = dest_parser_resultH (p a (mk_streamH s))`;;
+     drop_parser_functionH p =
+     \a s. drop_parser_resultH (p a (lift_streamH s))`;;
 
-export_thm dest_parseH_def;;
+export_thm drop_parser_functionH_def;;
 
-let abs_parserH_def = new_definition
+let mk_parserH_def = new_definition
   `!(p : A -> A streamH -> (B # A streamH) option).
-     abs_parserH p = mk_parserH (mk_parser (dest_parseH p))`;;
+     mk_parserH p = lift_parserH (mk_parser (drop_parser_functionH p))`;;
 
-export_thm abs_parserH_def;;
+export_thm mk_parserH_def;;
 
-let rep_parserH_def = new_definition
+let dest_parserH_def = new_definition
   `!(p : (A,B) parserH).
-     rep_parserH p = mk_parseH (dest_parser (dest_parserH p))`;;
+     dest_parserH p = lift_parser_functionH (dest_parser (drop_parserH p))`;;
 
-export_thm rep_parserH_def;;
+export_thm dest_parserH_def;;
+
+(* ------------------------------------------------------------------------- *)
+(* Properties of Haskell parsers and streams.                                *)
+(* ------------------------------------------------------------------------- *)
+
+logfile "haskell-parser-thm";;
+
+(* Parsers *)
+
+let parser_resultH_drop_lift = prove
+ (`!(r : (B # A stream) option).
+     drop_parser_resultH (lift_parser_resultH r) = r`,
+  GEN_TAC THEN
+  MP_TAC (ISPEC `r : (B # A stream) option` option_cases) THEN
+  STRIP_TAC THENL
+  [FIRST_X_ASSUM SUBST_VAR_TAC THEN
+   REWRITE_TAC [lift_parser_resultH_def; drop_parser_resultH_def];
+   ALL_TAC] THEN
+  FIRST_X_ASSUM SUBST_VAR_TAC THEN
+  MP_TAC (ISPEC `a : B # A stream` PAIR_SURJECTIVE) THEN
+  STRIP_TAC THEN
+  FIRST_X_ASSUM SUBST_VAR_TAC THEN
+  REWRITE_TAC
+    [lift_parser_resultH_def; drop_parser_resultH_def; streamH_drop_lift]);;
+
+export_thm parser_resultH_drop_lift;;
+
+let parser_functionH_drop_lift = prove
+ (`!(p : (A,B) parser).
+     drop_parser_functionH (lift_parser_functionH (dest_parser p)) =
+     dest_parser p`,
+  GEN_TAC THEN
+  CONV_TAC (REWR_CONV FUN_EQ_THM) THEN
+  X_GEN_TAC `a : A` THEN
+  CONV_TAC (REWR_CONV FUN_EQ_THM) THEN
+  X_GEN_TAC `s : A stream` THEN
+  REWRITE_TAC
+    [lift_parser_functionH_def; drop_parser_functionH_def;
+     streamH_drop_lift; parser_resultH_drop_lift]);;
+
+export_thm parser_functionH_drop_lift;;
+
+let parserH_mk_dest = prove
+ (`!(p : (A,B) parserH).
+     mk_parserH (dest_parserH p) = p`,
+  REWRITE_TAC
+    [mk_parserH_def; dest_parserH_def; parser_functionH_drop_lift;
+     parser_abs_rep; parserH_lift_drop]);;
+
+export_thm parserH_mk_dest;;
 
 (* ------------------------------------------------------------------------- *)
 (* A type of Haskell parsers.                                                *)
@@ -174,7 +208,7 @@ logfile "haskell-parser-src";;
 
 (* Streams *)
 
-let case_streamH_src = prove
+let () = (export_haskell_thm o prove)
  (`(!e b (f : A -> A streamH -> B). case_streamH e b f ErrorH = e) /\
    (!e b (f : A -> A streamH -> B). case_streamH e b f EofH = b) /\
    (!e b (f : A -> A streamH -> B) a s.
@@ -183,9 +217,7 @@ let case_streamH_src = prove
     [case_streamH_def; ErrorH_def; EofH_def; StreamH_def; case_stream_def;
      streamH_tybij]);;
 
-export_haskell_thm case_streamH_src;;
-
-let length_streamH_src = prove
+let () = (export_haskell_thm o prove)
  (`length_streamH (ErrorH : A streamH) = 0 /\
    length_streamH (EofH : A streamH) = 0 /\
    (!(a:A) s. length_streamH (StreamH a s) = length_streamH s + 1)`,
@@ -193,9 +225,7 @@ let length_streamH_src = prove
     [length_streamH_def; ErrorH_def; EofH_def; StreamH_def; streamH_tybij;
      length_stream_def; ADD1]);;
 
-export_haskell_thm length_streamH_src;;
-
-let stream_to_listH_src = prove
+let () = (export_haskell_thm o prove)
  (`stream_to_listH (ErrorH : A streamH) = NONE /\
    stream_to_listH (EofH : A streamH) = SOME [] /\
    (!(a : A) s.
@@ -205,26 +235,22 @@ let stream_to_listH_src = prove
     [stream_to_listH_def; ErrorH_def; EofH_def; StreamH_def; streamH_tybij;
      stream_to_list_def]);;
 
-export_haskell_thm stream_to_listH_src;;
-
-let append_streamH_src = prove
+let () = (export_haskell_thm o prove)
  (`(!(s : A streamH). append_streamH [] s = s) /\
    (!(h : A) t s.
       append_streamH (CONS h t) s = StreamH h (append_streamH t s))`,
   REWRITE_TAC
     [append_streamH_def; streamH_tybij; StreamH_def; append_stream_def]);;
 
-export_haskell_thm append_streamH_src;;
-
-let list_to_streamH_src = prove
+let () = (export_haskell_thm o prove)
  (`!(l : A list). list_to_streamH l = append_streamH l EofH`,
   REWRITE_TAC
     [list_to_streamH_def; streamH_tybij; EofH_def; list_to_stream_def;
      append_streamH_def]);;
 
-export_haskell_thm list_to_streamH_src;;
-
 (* Parsers *)
+
+let () = export_haskell_thm parserH_mk_dest;;
 
 (***
 export_haskell_thm (CONJUNCT1 parser_tybij);;
@@ -254,6 +280,7 @@ export_haskell_thm parse_option_def;;
 export_haskell_thm parse_some_def;;
 
 export_haskell_thm (REWRITE_RULE [FORALL_AND_THM] parse_stream_def);;
+***)
 
 (* ------------------------------------------------------------------------- *)
 (* Testing.                                                                  *)
@@ -263,13 +290,19 @@ logfile "haskell-parser-test";;
 
 (* Streams *)
 
+let () = (export_haskell_thm o prove)
+ (`!(l : A list) s.
+     length_streamH (append_streamH l s) = LENGTH l + length_streamH s`,
+  REWRITE_TAC
+    [length_streamH_def; append_streamH_def; streamH_drop_lift;
+     append_stream_length]);;
+
+(***
 export_haskell_thm append_stream_assoc;;
 
 export_haskell_thm list_to_stream_to_list;;
 
 export_haskell_thm stream_to_list_append;;
-
-export_haskell_thm append_stream_length;;
 
 export_haskell_thm list_to_stream_length;;
 
